fairness/actual_resources.v
@@ -4,7 +4,7 @@ From trillium.fairness Require Import fairness fuel fuel_ext resources partial_o
 
 
 Section actual_ownership.
-  Context `{LM: LiveModel G M}.
+  Context `{LM: LiveModel G M LSI_True}.
   Context `{Countable G}.
   (* Context `{EqDecision (expr Λ)}. *)
   Context {Σ : gFunctors}.
@@ -18,7 +18,7 @@ Section actual_ownership.
 End actual_ownership. 
 
 Section ActualOwnershipImpl.
-  Context `{LM: LiveModel G M}.
+  Context `{LM: LiveModel G M LSI_True}.
   Context `{Countable G}.
   (* Context `{EqDecision (expr Λ)}. *)
   Context {Σ : gFunctors}.
@@ -102,7 +102,7 @@ Section ActualOwnershipImpl.
     pose proof (SUB _ _ L1) as (S1'&?&?). pose proof (SUB _ _ L2) as (S2'&?&?).
     eapply disjoint_subseteq; eauto.
     apply _.
-  Qed. 
+  Qed.
 
   Lemma actual_update_no_step_enough_fuel
   (δ1: LM) rem
@@ -223,7 +223,10 @@ Proof.
       rewrite NEW_DOM.
       apply fuel_step_ls_tmap_dom; auto. }
 
-    iExists (build_LS_ext (ls_under δ1) _ Hfueldom (<[ζ:=dom fs ∖ rem]> (ls_tmap δ1 (LM := LM))) TMAP_DOM2 DISJ2 (LM := LM)).
+    (* assert (forall s m f, LSI_True s m f) as mk_LT. *)
+    (* { intros. rewrite /LSI_True.  *)
+
+    iExists (build_LS_ext (ls_under δ1) _ Hfueldom (<[ζ:=dom fs ∖ rem]> (ls_tmap δ1 (LM := LM))) TMAP_DOM2 DISJ2 ltac:(done) (LM := LM)).
 
     (* remember (build_LS_ext _ _ _ _ _ _) as δ2.  *)
     simpl.
@@ -480,7 +483,7 @@ Proof.
       1-8: (solve_disj δ1 ζ τ2 || solve_disj δ1 τ1 ζ || set_solver). 
       eapply (ls_tmap_disj δ1 τ1 τ2); eauto. }
 
-    iExists (build_LS_ext (ls_under δ1) _ Hfueldom _ TMAP2_DOM TMAP2_DISJ (LM := LM)).
+    iExists (build_LS_ext (ls_under δ1) _ Hfueldom _ TMAP2_DOM TMAP2_DISJ ltac:(done) (LM := LM)).
 
     iModIntro.
     assert (Hdomincl: dom fs ⊆ dom (ls_fuel δ1)).
@@ -606,7 +609,293 @@ Proof.
   (*   destruct (decide (x ∈ Y)); set_solver. *)
   (* Qed. *)
 
+  Lemma mim_model_step_helper
+    (s2 : M)
+    (fs1 fs2 : gmap (fmrole M) nat)
+    (ρ : fmrole M)
+    (δ1 : LM)
+    (ζ : G)
+    (fr1 : gset (fmrole M))
+    (Hfr_new : live_roles M s2 ∖ live_roles M (ls_under δ1) ⊆ fr1)
+    (Hfuelsval : valid_new_fuelmap fs1 fs2 (ls_under δ1) s2 ρ (LM := LM))
+    (Hxdom : ∀ ρ : fmrole M, ls_mapping δ1 !! ρ = Some ζ ↔ ρ ∈ dom fs1)
+    (HFR : fr1 ∩ dom (ls_fuel δ1) = ∅)
+:
+  maps_inverse_match
+    (map_imap
+       (λ (ρ' : fmrole M) (_ : nat),
+          if decide (ρ' ∈ dom (ls_fuel δ1)) then ls_mapping δ1 !! ρ' else Some ζ)
+       (gset_to_gmap 333 ((dom (ls_fuel δ1) ∪ dom fs2) ∖ (dom fs1 ∖ dom fs2))))
+    (<[ζ:=dom fs2]> (ls_tmap δ1 (LM := LM))). 
+  Proof.
+    intros ρ' ζ'. simpl. rewrite map_lookup_imap.
+    rewrite lookup_gset_to_gmap //=.
+    destruct (decide (ρ' ∈ (dom (ls_fuel δ1) ∪ dom fs2) ∖ (dom fs1 ∖ dom fs2))) as [Hin|Hnotin].
+    - rewrite option_guard_True //=. destruct (decide (ρ' ∈ dom (ls_fuel δ1))).
+      + destruct (decide (ζ' = ζ)) as [->|Hneq].
+        * rewrite lookup_insert. split.
+          { eexists; split =>//. apply elem_of_difference in Hin as [? Hin].
+            apply not_elem_of_difference in Hin as [?|?]; [|done].
+            set_solver. }
+          { intros (?&?&?). simplify_eq. apply Hxdom.
+            destruct Hfuelsval as (?&?&?&?&?). by_contradiction.
+            assert (ρ' ∈ live_roles M s2 ∖ live_roles M δ1).
+            { set_solver. }
+            assert (ρ' ∈ fr1).
+            { set_solver. }
+            assert (ρ' ∉ dom $ ls_fuel δ1) by set_solver .
+            done. }
+        * rewrite lookup_insert_ne //.
+          apply ls_mapping_tmap_corr.
+      + split.
+        * intros Htid. simplify_eq. rewrite lookup_insert. eexists; split=>//.
+          set_solver.
+        * assert (ρ' ∈ dom fs2) by set_solver. intros Hm. by_contradiction.
+          rewrite lookup_insert_ne in Hm; last congruence.
+          apply ls_mapping_tmap_corr in Hm.
+          apply elem_of_dom_2 in Hm. rewrite ls_same_doms // in Hm.
+    - destruct Hfuelsval as (?&?&?&?&Hinf&?). rewrite option_guard_False //=. split; first done.
+      destruct (decide (ζ' = ζ)) as [->|Hneq].
+      { rewrite lookup_insert //. intros (?&?&?). simplify_eq. set_solver. }
+      rewrite lookup_insert_ne //.
+      intros Habs%ls_mapping_tmap_corr.
+      
+      apply not_elem_of_difference in Hnotin as [Hnin|Hin].
+      + apply elem_of_dom_2 in Habs. rewrite ls_same_doms in Habs. set_solver.
+      + apply elem_of_difference in Hin as [Hin Hnin].
+        apply Hxdom in Hin. congruence.
+  Qed.
+
+  Lemma model_step_ls_trans
+  (s1 s2 : M)
+  (fs1 fs2 : gmap (fmrole M) nat)
+  (ρ : fmrole M)
+  (δ1 : LM)
+  (ζ : G)
+  (fr1 : gset (fmrole M))
+  (Hfr_new : live_roles M s2 ∖ live_roles M s1 ⊆ fr1)
+  (Htrans : fmtrans M s1 (Some ρ) s2)
+  (Hlim : ρ ∈ live_roles M s2 → oleq (fs2 !! ρ) (Some (lm_fl LM s2)))
+  (Hzombie : ρ ∉ live_roles M s2
+            → ρ ∈ dom fs1 ∩ dom fs2 → oleq (fs2 !! ρ) (fs1 !! ρ))
+  (Hinfs1m : ρ ∈ dom fs1)
+  (Hnewlim : ∀ ρ' : fmrole M,
+              ρ' ∈ dom fs2 ∖ dom fs1 → oleq (fs2 !! ρ') (Some (lm_fl LM s2)))
+  (Hdec : ∀ ρ' : fmrole M, ρ ≠ ρ' → ρ' ∈ dom fs1 ∩ dom fs2 → oless (fs2 !! ρ') (fs1 !! ρ'))
+  (Hinf : dom fs1 ∖ {[ρ]} ∪ live_roles M s2 ∖ live_roles M s1 ⊆ dom fs2)
+  (Hsup : dom fs2
+         ⊆ live_roles M s2 ∖ live_roles M s1
+           ∪ (live_roles M s2 ∩ live_roles M s1) ∩ dom fs1
+           ∪ dom fs1 ∖ live_roles M s1
+           ∪ (live_roles M s1 ∖ live_roles M s2) ∩ dom fs1)
+  (Hxdom : ∀ ρ : fmrole M, ls_mapping δ1 !! ρ = Some ζ ↔ ρ ∈ dom fs1)
+  (Hfuel : ∀ ρ : fmrole M, ρ ∈ dom fs1 → ls_fuel δ1 !! ρ = fs1 !! ρ)
+  (FR : gset (fmrole M))
+  (HFR : FR ∩ dom (ls_fuel δ1) = ∅)
+  (Heq : ls_under δ1 = s1)
+  (HfrFR : fr1 ⊆ FR)
+  (new_mapping := map_imap
+                   (λ (ρ' : fmrole M) (_ : nat),
+                      if decide (ρ' ∈ dom (ls_fuel δ1))
+                      then ls_mapping δ1 !! ρ'
+                      else Some ζ)
+                   (gset_to_gmap 333
+                      ((dom (ls_fuel δ1) ∪ dom fs2) ∖ (dom fs1 ∖ dom fs2))))
+  (Hsamedoms : dom new_mapping = dom (update_fuel_resource δ1 fs1 fs2 s2))
+  (Hnewdom : dom (update_fuel_resource δ1 fs1 fs2 s2) =
+            (dom (ls_fuel δ1) ∪ dom fs2) ∖ (dom fs1 ∖ dom fs2))
+  (Hfueldom : live_roles M s2 ⊆ dom (update_fuel_resource δ1 fs1 fs2 s2))
+  (FR' : gset (fmrole M))
+  (FR_EQ : FR = fr1 ∪ FR')
+  (DISJ' : fr1 ## FR')
+  (MATCH : maps_inverse_match new_mapping (<[ζ:=dom fs2]> (ls_tmap δ1 (LM := LM))))
+:
+    forall tmap_sd tmap_disj,
+  lm_ls_trans LM δ1 (Take_step ρ ζ)
+    (build_LS_ext s2 (update_fuel_resource δ1 fs1 fs2 s2) Hfueldom
+       (<[ζ:=dom fs2]> (ls_tmap δ1 (LM := LM)))
+       tmap_sd tmap_disj I (LM := LM)). 
+  Proof.
+    intros. 
+    constructor; simpl.
+    { rewrite build_LS_ext_spec_st. by rewrite Heq //. }
+    split; first by apply Hxdom; set_solver.
+    split.
+    { intros ? ? Hdom Hmd. 
+      rewrite build_LS_ext_spec_fuel. erewrite build_LS_ext_spec_fuel in *. 
+      inversion Hmd; clear Hmd; simplify_eq.
+      + symmetry in Hsametid. rewrite -> Hxdom in Hsametid. simpl.
+        unfold update_fuel_resource, fuel_apply.
+        rewrite map_lookup_imap lookup_gset_to_gmap.
+        destruct (decide (ρ' ∈ live_roles M s2 ∪ dom fs2)) as [Hin|Hin].
+        * rewrite option_guard_True //=.
+          { destruct (decide (ρ' ∈ dom fs2)) as [Hin2|Hin2].
+            ** rewrite Hfuel; last set_solver.
+               apply Hdec; [congruence|set_solver -Hsamedoms Hnewdom Hdom].
+            ** exfalso. set_solver -Hsamedoms Hnewdom Hdom. }
+          apply elem_of_difference; split;
+            [set_solver -Hsamedoms Hnewdom Hdom|].
+          apply not_elem_of_difference; right.
+          apply elem_of_union in Hin as [|]; [|done].
+          destruct (decide (ρ' = ρ)); simplify_eq.
+          apply Hinf; set_solver -Hsamedoms Hnewdom Hdom.
+        * rewrite option_guard_False //=.
+          ** assert (ρ' ∈ dom fs2); set_solver -Hsamedoms Hnewdom Hdom.
+          ** apply not_elem_of_difference; right; set_solver -Hsamedoms Hnewdom Hdom.
+      + simpl in *. unfold update_fuel_resource, fuel_apply.
+        rewrite map_lookup_imap lookup_gset_to_gmap.
+        
+        erewrite build_LS_ext_spec_mapping in Hneqtid, Hissome.
+        2, 3: by eauto.
+        destruct (decide (ρ' ∈ (dom (ls_fuel δ1) ∪ dom fs2) ∖ (dom fs1 ∖ dom fs2))) as [Hin|Hin].
+        * rewrite map_lookup_imap lookup_gset_to_gmap option_guard_True //= decide_True //= in Hneqtid.
+        * apply not_elem_of_difference in Hin as [?|Hin];
+            [set_solver -Hsamedoms Hnewdom Hdom|].
+          apply elem_of_difference in Hin as [??].
+          rewrite map_lookup_imap lookup_gset_to_gmap /= option_guard_False /= in Hissome;
+            [inversion Hissome; congruence|set_solver -Hsamedoms Hnewdom Hdom]. }
+    split.
+    + intros ? Hin.
+      rewrite build_LS_ext_spec_fuel build_LS_ext_spec_st. 
+      simplify_eq; simpl.
+      
+      unfold update_fuel_resource, fuel_apply.
+      rewrite map_lookup_imap lookup_gset_to_gmap.
+      destruct (decide (ρ' ∈ (dom (ls_fuel δ1) ∪ dom fs2) ∖ (dom fs1 ∖ dom fs2))) as [Hlive|Hlive].
+      * rewrite option_guard_True //=.
+        apply elem_of_difference in Hlive as [Hin1 Hnin].
+        apply not_elem_of_difference in Hnin.
+        destruct (decide (ρ' ∈ dom fs2)) as [Hin2|Hin2].
+        **
+          destruct (decide (ρ' = ρ)).
+          { subst ρ'. destruct Hnin; [set_solver| ].
+            destruct (decide (ρ ∈ live_roles M s2)).
+            - tauto.
+            - left. rewrite Hfuel; set_solver. }
+          destruct (decide (ρ' ∈ live_roles _ δ1)); left.
+          *** destruct (decide (ρ' ∈ dom fs1)).
+              { rewrite Hfuel //.
+                apply oleq_oless, Hdec; [congruence|set_solver -Hsamedoms Hnewdom]. }
+              { exfalso. set_solver -Hsamedoms Hnewdom. }
+          *** assert (ρ' ∉ live_roles _ s2).
+              { by_contradiction. assert (ρ' ∈ fr1); [eapply elem_of_subseteq; eauto; set_solver -Hsamedoms Hnewdom|].
+                assert (ρ' ∈ (fr1 ∪ FR')); [eapply elem_of_subseteq; eauto; set_solver -Hsamedoms Hnewdom|set_solver -Hsamedoms Hnewdom]. }
+                    assert (ρ' ∈ dom fs1) by set_solver -Hsamedoms Hnewdom.
+              rewrite Hfuel //. apply oleq_oless, Hdec; [congruence|set_solver -Hsamedoms Hnewdom].
+        ** left. rewrite elem_of_dom in Hin. destruct Hin as [? ->]. simpl;lia.
+      * destruct (decide (ρ' = ρ)).
+        { subst. right. left. split; auto. left.               
+          eapply not_elem_of_weaken; [|by apply map_imap_dom_inclusion; rewrite dom_gset_to_gmap].
+          rewrite dom_gset_to_gmap //. }
+        
+        right; right; split.
+        ** eapply not_elem_of_weaken; [|by apply map_imap_dom_inclusion; rewrite dom_gset_to_gmap].
+           rewrite dom_gset_to_gmap //.
+        ** apply not_elem_of_difference in Hlive as [?|Hlive]; [set_solver -Hsamedoms Hnewdom|].
+           apply elem_of_difference in Hlive as [? Habs].
+           exfalso. apply Habs.
+           set_solver -Hsamedoms Hnewdom Hfueldom.
+    +
+      rewrite build_LS_ext_spec_fuel build_LS_ext_spec_st.
+      split.
+      { intros Hlive.
+        
+        unfold update_fuel_resource, fuel_apply.
+        destruct (decide (ρ ∈ (dom (ls_fuel δ1) ∪ dom fs2) ∖ (dom fs1 ∖ dom fs2))) as [Hin|Hnin].
+        - rewrite map_lookup_imap lookup_gset_to_gmap option_guard_True //=.
+          rewrite decide_True; [by apply Hlim |set_solver -Hsamedoms Hnewdom Hfueldom].
+        - exfalso; apply not_elem_of_difference in Hnin as [Hnin|Hnin].
+          + assert (ρ ∉ live_roles _ δ1).
+            eapply not_elem_of_weaken => //.
+            { epose proof ls_fuel_dom. set_solver -Hsamedoms Hnewdom Hfueldom. }
+            assert (ρ ∈ dom fs2) by set_solver -Hsamedoms Hnewdom Hfueldom. set_solver -Hsamedoms Hnewdom Hfueldom.
+          + apply elem_of_difference in Hnin as [? Hnin].
+            apply not_elem_of_dom in Hnin. rewrite Hnin /= in Hlim.
+            by apply Hlim. }
+      split.
+      { intros ρ'. unfold update_fuel_resource, fuel_apply => Hin.
+        rewrite map_imap_dom_eq in Hin; last first.
+        { intros ρ0 _ Hin'. destruct (decide (ρ0 ∈ dom fs2)); [by apply elem_of_dom|].
+          rewrite dom_gset_to_gmap elem_of_difference in Hin'.
+          destruct Hin' as [Hin' ?]. apply elem_of_union in Hin' as [?|?]; [by apply elem_of_dom|done]. }
+        rewrite dom_gset_to_gmap in Hin. rewrite map_lookup_imap lookup_gset_to_gmap option_guard_True /=; last set_solver -Hsamedoms Hnewdom Hfueldom.
+        assert (ρ' ∈ dom fs2) by set_solver -Hsamedoms Hnewdom Hfueldom. rewrite decide_True //. apply Hnewlim. apply elem_of_difference; split =>//.
+        intros contra%Hxdom%elem_of_dom_2. rewrite ls_same_doms in contra. simplify_eq. set_solver -Hsamedoms Hnewdom Hfueldom. }
+      intros ρ0 Hin.
+      assert (ρ0 ∉ live_roles _ δ1).
+      { eapply not_elem_of_weaken; last apply ls_fuel_dom. set_solver -Hsamedoms Hnewdom Hfueldom. }
+      apply elem_of_difference in Hin as [Hin1 Hnin].
+      assert (ρ0 ∈ live_roles _ s2).
+      { by_contradiction.
+        assert (ρ0 ∈ dom fs2).
+        { unfold update_fuel_resource, fuel_apply in Hin1.
+          eapply elem_of_subseteq in Hin1; last apply map_imap_dom_inclusion.
+          rewrite dom_gset_to_gmap in Hin1. set_solver -Hsamedoms Hnewdom Hfueldom. }
+        exfalso. assert (Hinabs: ρ0 ∈ dom fs1) by set_solver -Hsamedoms Hnewdom Hfueldom.
+        apply not_elem_of_dom in Hnin. rewrite Hfuel // in Hnin.
+        apply elem_of_dom in Hinabs. rewrite Hnin in Hinabs. simpl in Hinabs.
+        by inversion Hinabs. }
+      set_solver -Hsamedoms Hnewdom Hfueldom.
+  Qed. 
+
+  Lemma model_step_new_fr
+  (s1 s2 : M)
+  (fs1 fs2 : gmap (fmrole M) nat)
+  (ρ : fmrole M)
+  (δ1 : LM)
+  (ζ : G)
+  (fr1 fr_stash : gset (fmrole M))
+  (Hfr_new : live_roles M s2 ∖ live_roles M s1 ⊆ fr1)
+  (Hstash_own : fr_stash ⊆ dom fs1)
+  (Hstash_dis : live_roles M s1 ∩ (fr_stash ∖ {[ρ]}) = ∅)
+  (Hstash_rem : dom fs2 ∩ fr_stash = ∅)
+  (Hfuelsval : valid_new_fuelmap fs1 fs2 s1 s2 ρ (LM := LM))
+  (* (Hfsne : fs1 ≠ ∅) *)
+  (Hxdom : ∀ ρ : fmrole M, ls_mapping δ1 !! ρ = Some ζ ↔ ρ ∈ dom fs1)
+  (Hfuel : ∀ ρ : fmrole M, ρ ∈ dom fs1 → ls_fuel δ1 !! ρ = fs1 !! ρ)
+  (FR : gset (fmrole M))
+  (HFR : FR ∩ dom (ls_fuel δ1) = ∅)
+  (Heq : ls_under δ1 = s1)
+  (HfrFR : fr1 ⊆ FR)
+  (FR' : gset (fmrole M))
+  (FR_EQ : FR = fr1 ∪ FR')
+  (DISJ' : fr1 ## FR')
+  :
+  (fr1 ∖ (live_roles M s2 ∖ live_roles M s1) ∪ fr_stash ∪ FR')
+   ∩ dom (update_fuel_resource δ1 fs1 fs2 s2) = ∅.
+  Proof. 
+    simpl. rewrite /update_fuel_resource /fuel_apply.
+    rewrite map_imap_dom_eq ?dom_gset_to_gmap.
+    2: { intros ρ' _ Hin. destruct (decide (ρ' ∈ dom fs2)) as [Hin'|].
+         { apply elem_of_dom in Hin' as [? ->]. done. }
+         assert (ρ' ∈ dom (ls_fuel δ1)) as Hin' by set_solver. 
+         apply elem_of_dom in  Hin' as [? ->]. done. }
+
+    apply elem_of_equiv_empty_L. intros ρ' [Hin1 Hin2]%elem_of_intersection.
+      
+    (* TODO: problems with elem_of_proper *)
+    assert (fr1 ∖ (live_roles M s2 ∖ live_roles M s1) ∪ fr_stash ∪ FR' ≡ FR ∖ (live_roles M s2 ∖ live_roles M s1) ∪ fr_stash ∪ FR' ∩ (live_roles M s2 ∖ live_roles M s1)) as ALT.
+    { set_solver -Hin1 Hin2. }
+    rewrite ALT in Hin1. clear ALT. 
     
+    apply elem_of_union in Hin1 as [[Hin1 | Hin1] %elem_of_union | Hin1].
+    2, 3: set_solver.
+    apply elem_of_difference in Hin1 as [Hin11 Hin12].
+    apply not_elem_of_difference in Hin12.
+    apply elem_of_difference in Hin2 as [Hin21 Hin22].
+    apply not_elem_of_difference in Hin22.
+    assert (ρ' ∉ dom $ ls_fuel δ1) by set_solver.
+    assert (ρ' ∈ dom fs2) by set_solver.
+    destruct Hin12 as [Hin12|Hin12].
+    2: { eapply H0. eapply ls_fuel_dom. set_solver. }
+    destruct Hfuelsval as (?&?&?&?&?&?).
+    assert (ρ' ∉ dom fs1).
+    2: { eapply H0. eapply ls_fuel_dom. set_solver -Hin11 Hin21 Hin22. }
+    intros contra. pose proof (Hfuel _ contra) as Habs. apply elem_of_dom in contra as [? contra].
+    rewrite contra in Habs. apply elem_of_dom_2 in Habs. done.
+  Qed.
+    
+   
   Lemma actual_update_step_still_alive
         s1 s2 fs1 fs2 ρ (δ1 : LM) ζ fr1 fr_stash:
     (live_roles _ s2 ∖ live_roles _ s1) ⊆ fr1 ->
@@ -649,7 +938,7 @@ Proof.
           rewrite decide_True //. apply elem_of_dom. rewrite Hin1; eauto.
           rewrite map_imap_dom_eq dom_gset_to_gmap in Hin; first set_solver.
           intros ρ0??. destruct (decide (ρ0 ∈ dom $ ls_fuel δ1)); [|done].
-          apply elem_of_dom. rewrite ls_same_doms. SS.
+          apply elem_of_dom. by rewrite ls_same_doms.
         + rewrite map_imap_dom_eq dom_gset_to_gmap; last first.
           { intros ρ0 ? Hin0. destruct (decide (ρ0 ∈ dom fs2)) as [|Hnotin]; apply elem_of_dom; first done.
             unfold valid_new_fuelmap in Hfuelsval.
@@ -657,12 +946,12 @@ Proof.
 
           rewrite map_imap_dom_eq dom_gset_to_gmap in Hin; first set_solver.
           intros ρ0??. destruct (decide (ρ0 ∈ dom $ ls_fuel δ1)); [|done].
-          apply elem_of_dom. rewrite ls_same_doms. SS.
+          apply elem_of_dom. by rewrite ls_same_doms. 
       - intros [f Hin]%elem_of_dom. rewrite map_lookup_imap in Hin.
         rewrite map_imap_dom_eq dom_gset_to_gmap.
         + by_contradiction. rewrite lookup_gset_to_gmap option_guard_False // in Hin.
         + intros ρ0??. destruct (decide (ρ0 ∈ dom $ ls_fuel δ1)); [|done].
-          apply elem_of_dom. rewrite ls_same_doms. SS. }
+          apply elem_of_dom. by rewrite ls_same_doms. }
 
     assert (Hnewdom: dom (update_fuel_resource δ1 fs1 fs2 s2) =
                        (dom (ls_fuel δ1) ∪ dom fs2) ∖ (dom fs1 ∖ dom fs2)).
@@ -686,7 +975,7 @@ Proof.
           split; [apply elem_of_union; right; set_unfold; naive_solver|
                    set_unfold; naive_solver]. }
       intros ρ0??. destruct (decide (ρ0 ∈ dom $ ls_fuel δ1)); [|done].
-      apply elem_of_dom. rewrite ls_same_doms. SS. }
+      apply elem_of_dom. by rewrite ls_same_doms. }
     (* iExists {| *)
     (*   ls_under := s2; *)
     (*   ls_fuel :=  _; *)
@@ -694,7 +983,7 @@ Proof.
     (*   ls_mapping := _; *)
     (*   ls_same_doms := Hsamedoms; *)
     (* |}.  *)
-    iExists (build_LS_ext s2 _ Hfueldom (<[ζ:=dom fs2]> (ls_tmap δ1 (LM := LM))) _ _ (LM := LM)).
+    iExists (build_LS_ext s2 _ Hfueldom (<[ζ:=dom fs2]> (ls_tmap δ1 (LM := LM))) _ _ ltac:(done) (LM := LM)).
     (* Unshelve. *)
     iMod (update_has_fuels _ fs1 fs2 with "Hfuel Hafuel Hamapping") as "(Hafuel & Hfuel & Hmapping)".
     { set_solver. }
@@ -732,219 +1021,25 @@ Proof.
     { by rewrite FR_EQ. }
     
     assert (maps_inverse_match new_mapping (<[ζ:=dom fs2]> (ls_tmap δ1 (LM := LM)))) as MATCH.
-    { subst new_mapping s1 FR. 
-      clear -Hxdom Hfuelsval fr1 Hfr_new FR' HFR.
-      
-      intros ρ' ζ'. simpl. rewrite map_lookup_imap.
-      rewrite lookup_gset_to_gmap //=.
-      destruct (decide (ρ' ∈ (dom (ls_fuel δ1) ∪ dom fs2) ∖ (dom fs1 ∖ dom fs2))) as [Hin|Hnotin].
-      - rewrite option_guard_True //=. destruct (decide (ρ' ∈ dom (ls_fuel δ1))).
-        + destruct (decide (ζ' = ζ)) as [->|Hneq].
-          * rewrite lookup_insert. split.
-            { eexists; split =>//. apply elem_of_difference in Hin as [? Hin].
-              apply not_elem_of_difference in Hin as [?|?]; [|done].
-              set_solver. }
-            { intros (?&?&?). simplify_eq. apply Hxdom.
-              destruct Hfuelsval as (?&?&?&?&?). by_contradiction.
-              assert (ρ' ∈ live_roles M s2 ∖ live_roles M δ1).
-              { set_solver. }
-               assert (ρ' ∈ fr1).
-              { set_solver. }
-              assert (ρ' ∈ (fr1 ∪ FR')) by set_solver.
-              assert (ρ' ∉ dom $ ls_fuel δ1) by set_solver .
-              done. }
-          * rewrite lookup_insert_ne //.
-            apply ls_mapping_tmap_corr.
-        + split.
-          * intros Htid. simplify_eq. rewrite lookup_insert. eexists; split=>//.
-            set_solver.
-          * assert (ρ' ∈ dom fs2) by set_solver. intros Hm. by_contradiction.
-            rewrite lookup_insert_ne in Hm; last congruence.
-            apply ls_mapping_tmap_corr in Hm.
-            apply elem_of_dom_2 in Hm. rewrite ls_same_doms // in Hm.
-      - destruct Hfuelsval as (?&?&?&?&Hinf&?). rewrite option_guard_False //=. split; first done.
-        destruct (decide (ζ' = ζ)) as [->|Hneq].
-        { rewrite lookup_insert //. intros (?&?&?). simplify_eq. set_solver. }
-        rewrite lookup_insert_ne //.
-        intros Habs%ls_mapping_tmap_corr.
-
-        apply not_elem_of_difference in Hnotin as [Hnin|Hin].
-        + apply elem_of_dom_2 in Habs. rewrite ls_same_doms in Habs. set_solver.
-        + apply elem_of_difference in Hin as [Hin Hnin].
-          apply Hxdom in Hin. congruence. }
+    { eapply @mim_model_step_helper; eauto.
+      { rewrite Heq. apply Hfuelsval. }
+      rewrite Heq; eauto.
+      clear -Hfr_new HFR HfrFR. set_solver. }
 
     iModIntro.
     iSplit.
     { iPureIntro.
       destruct Hfuelsval as (Hlim&Hzombie&Hinfs1m&Hnewlim&Hdec&Hinf&Hsup).
-      (* constructor =>//.  *)
-      - constructor; simpl.
-        { rewrite build_LS_ext_spec_st. by rewrite Heq //. }
-        split; first by apply Hxdom; set_solver.
-        split.
-        { intros ? ? Hdom Hmd. inversion Hmd; clear Hmd; simplify_eq.
-          + symmetry in Hsametid. rewrite -> Hxdom in Hsametid. simpl.
-            unfold update_fuel_resource, fuel_apply.
-            rewrite build_LS_ext_spec_fuel.
-            rewrite map_lookup_imap lookup_gset_to_gmap.
-            destruct (decide (ρ' ∈ live_roles M s2 ∪ dom fs2)) as [Hin|Hin].
-            * rewrite option_guard_True //=.
-              { destruct (decide (ρ' ∈ dom fs2)) as [Hin2|Hin2].
-                ** rewrite Hfuel; last set_solver.
-                   apply Hdec; [congruence|set_solver -Hsamedoms Hnewdom Hdom].
-                ** exfalso. set_solver -Hsamedoms Hnewdom Hdom. }
-              apply elem_of_difference; split;
-                [set_solver -Hsamedoms Hnewdom Hdom|].
-              apply not_elem_of_difference; right.
-              apply elem_of_union in Hin as [|]; [|done].
-              destruct (decide (ρ' = ρ)); simplify_eq.
-              apply Hinf; set_solver -Hsamedoms Hnewdom Hdom.
-            * rewrite option_guard_False //=.
-              ** assert (ρ' ∈ dom fs2); set_solver -Hsamedoms Hnewdom Hdom.
-              ** apply not_elem_of_difference; right; set_solver -Hsamedoms Hnewdom Hdom.
-          + simpl in *. unfold update_fuel_resource, fuel_apply.
-            rewrite build_LS_ext_spec_fuel.
-            rewrite map_lookup_imap lookup_gset_to_gmap.
-
-            erewrite build_LS_ext_spec_mapping in Hneqtid, Hissome.
-            2, 3: by eauto.
-            destruct (decide (ρ' ∈ (dom (ls_fuel δ1) ∪ dom fs2) ∖ (dom fs1 ∖ dom fs2))) as [Hin|Hin].
-            * rewrite map_lookup_imap lookup_gset_to_gmap option_guard_True //= decide_True //= in Hneqtid.
-            * apply not_elem_of_difference in Hin as [?|Hin];
-                [set_solver -Hsamedoms Hnewdom Hdom|].
-              apply elem_of_difference in Hin as [??].
-              rewrite map_lookup_imap lookup_gset_to_gmap /= option_guard_False /= in Hissome;
-                [inversion Hissome; congruence|set_solver -Hsamedoms Hnewdom Hdom].
-          (* + simpl in *. rewrite Hfuel; last set_solver -Hsamedoms Hnewdom Hdom. *)
-          (*   unfold update_fuel_resource, fuel_apply. *)
-          (*   rewrite build_LS_ext_spec_fuel in Hnotdead, Hdom. *)
-          (*   rewrite Hnewdom in Hnotdead. *)
-          (*   rewrite build_LS_ext_spec_fuel. *)
-          (*   rewrite map_lookup_imap lookup_gset_to_gmap option_guard_True //=. *)
-          (*   assert (ρ' ∈ dom fs2) by (set_solver -Hsamedoms Hnewdom Hdom). *)
-          (*   rewrite decide_True; [| done]. *)
-          (*   apply Hzombie =>//; [| set_solver]. *)
-          (*   rewrite build_LS_ext_spec_st in Hnotalive. *)
-          (*   set_solver -Hsamedoms Hnewdom Hdom. *)
-    }
-        split.
-        + intros ? Hin.
-          rewrite build_LS_ext_spec_fuel build_LS_ext_spec_st. 
-          simplify_eq; simpl.
-
-          unfold update_fuel_resource, fuel_apply.
-          rewrite map_lookup_imap lookup_gset_to_gmap.
-          destruct (decide (ρ' ∈ (dom (ls_fuel δ1) ∪ dom fs2) ∖ (dom fs1 ∖ dom fs2))) as [Hlive|Hlive].
-          * rewrite option_guard_True //=.
-            apply elem_of_difference in Hlive as [Hin1 Hnin].
-            apply not_elem_of_difference in Hnin.
-            destruct (decide (ρ' ∈ dom fs2)) as [Hin2|Hin2].
-            **
-              destruct (decide (ρ' = ρ)).
-              { subst ρ'. destruct Hnin; [set_solver| ].
-                destruct (decide (ρ ∈ live_roles M s2)).
-                - tauto.
-                - left. rewrite Hfuel; set_solver. }
-              destruct (decide (ρ' ∈ live_roles _ δ1)); left.
-               *** destruct (decide (ρ' ∈ dom fs1)).
-                   { rewrite Hfuel //.
-                     apply oleq_oless, Hdec; [congruence|set_solver -Hsamedoms Hnewdom]. }
-                   { exfalso. set_solver -Hsamedoms Hnewdom. }
-               *** assert (ρ' ∉ live_roles _ s2).
-                   { by_contradiction. assert (ρ' ∈ fr1); [eapply elem_of_subseteq; eauto; set_solver -Hsamedoms Hnewdom|].
-                     assert (ρ' ∈ (fr1 ∪ FR')); [eapply elem_of_subseteq; eauto; set_solver -Hsamedoms Hnewdom|set_solver -Hsamedoms Hnewdom]. }
-                   assert (ρ' ∈ dom fs1) by set_solver -Hsamedoms Hnewdom.
-                   rewrite Hfuel //. apply oleq_oless, Hdec; [congruence|set_solver -Hsamedoms Hnewdom].
-            ** left. rewrite elem_of_dom in Hin. destruct Hin as [? ->]. simpl;lia.
-          * destruct (decide (ρ' = ρ)).
-            { subst. right. left. split; auto. left.               
-              eapply not_elem_of_weaken; [|by apply map_imap_dom_inclusion; rewrite dom_gset_to_gmap].
-              rewrite dom_gset_to_gmap //. }
-
-            right; right; split.
-            ** eapply not_elem_of_weaken; [|by apply map_imap_dom_inclusion; rewrite dom_gset_to_gmap].
-               rewrite dom_gset_to_gmap //.
-            ** apply not_elem_of_difference in Hlive as [?|Hlive]; [set_solver -Hsamedoms Hnewdom|].
-               apply elem_of_difference in Hlive as [? Habs].
-               exfalso. apply Habs.
-               set_solver -Hsamedoms Hnewdom Hfueldom.
-        +
-          rewrite build_LS_ext_spec_fuel build_LS_ext_spec_st.
-          split.
-          { intros Hlive.
-            
-            unfold update_fuel_resource, fuel_apply.
-          destruct (decide (ρ ∈ (dom (ls_fuel δ1) ∪ dom fs2) ∖ (dom fs1 ∖ dom fs2))) as [Hin|Hnin].
-          - rewrite map_lookup_imap lookup_gset_to_gmap option_guard_True //=.
-            rewrite decide_True; [by apply Hlim |set_solver -Hsamedoms Hnewdom Hfueldom].
-          - exfalso; apply not_elem_of_difference in Hnin as [Hnin|Hnin].
-            + assert (ρ ∉ live_roles _ δ1).
-              eapply not_elem_of_weaken => //.
-              { epose proof ls_fuel_dom. set_solver -Hsamedoms Hnewdom Hfueldom. }
-              assert (ρ ∈ dom fs2) by set_solver -Hsamedoms Hnewdom Hfueldom. set_solver -Hsamedoms Hnewdom Hfueldom.
-            + apply elem_of_difference in Hnin as [? Hnin].
-              apply not_elem_of_dom in Hnin. rewrite Hnin /= in Hlim.
-              by apply Hlim. }
-          split.
-          { intros ρ'. unfold update_fuel_resource, fuel_apply => Hin.
-            rewrite map_imap_dom_eq in Hin; last first.
-            { intros ρ0 _ Hin'. destruct (decide (ρ0 ∈ dom fs2)); [by apply elem_of_dom|].
-              rewrite dom_gset_to_gmap elem_of_difference in Hin'.
-              destruct Hin' as [Hin' ?]. apply elem_of_union in Hin' as [?|?]; [by apply elem_of_dom|done]. }
-            rewrite dom_gset_to_gmap in Hin. rewrite map_lookup_imap lookup_gset_to_gmap option_guard_True /=; last set_solver -Hsamedoms Hnewdom Hfueldom.
-            assert (ρ' ∈ dom fs2) by set_solver -Hsamedoms Hnewdom Hfueldom. rewrite decide_True //. apply Hnewlim. apply elem_of_difference; split =>//.
-            intros contra%Hxdom%elem_of_dom_2. rewrite ls_same_doms in contra. simplify_eq. set_solver -Hsamedoms Hnewdom Hfueldom. }
-          intros ρ0 Hin.
-          assert (ρ0 ∉ live_roles _ δ1).
-          { eapply not_elem_of_weaken; last apply ls_fuel_dom. set_solver -Hsamedoms Hnewdom Hfueldom. }
-          apply elem_of_difference in Hin as [Hin1 Hnin].
-          assert (ρ0 ∈ live_roles _ s2).
-          { by_contradiction.
-            assert (ρ0 ∈ dom fs2).
-            { unfold update_fuel_resource, fuel_apply in Hin1.
-              eapply elem_of_subseteq in Hin1; last apply map_imap_dom_inclusion.
-              rewrite dom_gset_to_gmap in Hin1. set_solver -Hsamedoms Hnewdom Hfueldom. }
-            exfalso. assert (Hinabs: ρ0 ∈ dom fs1) by set_solver -Hsamedoms Hnewdom Hfueldom.
-            apply not_elem_of_dom in Hnin. rewrite Hfuel // in Hnin.
-            apply elem_of_dom in Hinabs. rewrite Hnin in Hinabs. simpl in Hinabs.
-            by inversion Hinabs. }
-          set_solver -Hsamedoms Hnewdom Hfueldom. }
+      eapply model_step_ls_trans; eauto. }
 
     iFrame "Hfuel Hmod Hfr2".
     iSplitL; [| rewrite build_LS_ext_spec_tmap; done]. 
 
     iExists _.
     rewrite build_LS_ext_spec_st build_LS_ext_spec_fuel build_LS_ext_spec_tmap.
-    iFrame. all: eauto. (* TODO: find source... *)
-        
-
-    { simpl. rewrite /update_fuel_resource /fuel_apply.
-      rewrite map_imap_dom_eq ?dom_gset_to_gmap.
-      + iPureIntro. 
-        apply elem_of_equiv_empty_L. intros ρ' [Hin1 Hin2]%elem_of_intersection.
-
-        (* TODO: problems with elem_of_proper *)
-        assert (fr1 ∖ (live_roles M s2 ∖ live_roles M s1) ∪ fr_stash ∪ FR' ≡ FR ∖ (live_roles M s2 ∖ live_roles M s1) ∪ fr_stash ∪ FR' ∩ (live_roles M s2 ∖ live_roles M s1)) as ALT.
-        { set_solver. }
-        rewrite ALT in Hin1.
-
-        apply elem_of_union in Hin1 as [[Hin1 | Hin1] %elem_of_union | Hin1].
-        2, 3: set_solver.
-        apply elem_of_difference in Hin1 as [Hin11 Hin12].
-        apply not_elem_of_difference in Hin12.
-        apply elem_of_difference in Hin2 as [Hin21 Hin22].
-        apply not_elem_of_difference in Hin22.
-        assert (ρ' ∉ dom $ ls_fuel δ1) by set_solver -Hsamedoms Hnewdom Hfueldom.
-        assert (ρ' ∈ dom fs2) by set_solver -Hsamedoms Hnewdom Hfueldom.
-        destruct Hin12 as [Hin12|Hin12]; last by (epose proof ls_fuel_dom; set_solver -Hsamedoms Hnewdom Hfueldom).
-        destruct Hfuelsval as (?&?&?&?&?&?).
-        assert (ρ' ∉ dom fs1); last set_solver -Hsamedoms Hnewdom Hfueldom.
-        intros contra. pose proof (Hfuel _ contra) as Habs. apply elem_of_dom in contra as [? contra].
-        rewrite contra in Habs. apply elem_of_dom_2 in Habs. done.
-    + intros ρ' _ Hin. destruct (decide (ρ' ∈ dom fs2)) as [Hin'|].
-      * apply elem_of_dom in Hin' as [? ->]. done.
-      * assert (ρ' ∈ dom (ls_fuel δ1)) as Hin' by set_solver -Hsamedoms Hnewdom Hfueldom. apply elem_of_dom in Hin' as [? ->]. done. }
-
+    iFrame. all: eauto. (* TODO: find source... *)        
+    { iPureIntro. eapply model_step_new_fr; eauto. }
+    
     Unshelve. all: eauto.
     - intros. 
       rewrite Hnewdom. setoid_rewrite lookup_insert_Some.
@@ -996,7 +1091,7 @@ Proof.
       + inversion H1. subst. symmetry. eapply FS2_DISJ; eauto.
       + assert (τ1 ≠ τ2) by congruence. 
         eapply ls_tmap_disj; eauto. 
-  Qed. 
+  Qed.
 
 
 End ActualOwnershipImpl.
